\documentclass[preview]{standalone}
\usepackage{semantic}
\begin{document}
\[
  \inference[apply-unary]{
    F, D, L \vdash e : \langle d_1, d_2, R_1 \rangle \\
    ((\tau_p) \rightarrow \tau_r) := F[f] \\ 
    \langle 1, 1, R_1 \rangle := \tau_p & \langle 1, 1, R_2 \rangle := \tau_r \\
  }{
    F, D, L \vdash \texttt{apply(} f \texttt{, } e \texttt{)} : \langle d_1, d_2, R_2 \rangle
  }
\]

\[
  \inference[apply-binary]{
    F, D, L \vdash e_1 : \langle d_1, d_2, R_1 \rangle \\
    F, D, L \vdash e_2 : \langle 1, 1, R_2 \rangle \\
    ((\tau_{p_1} \times \tau_{p_2}) \rightarrow \tau_r) := F[f] \\ 
    \langle 1, 1, R_1 \rangle := \tau_{p_1} 
      & \langle 1, 1, R_2 \rangle := \tau_{p_2} 
      & \langle 1, 1, R_3 \rangle := \tau_r \\
  }{
    F, D, L \vdash \texttt{apply(} f \texttt{, } e_1 \texttt{, } e_2 \texttt{)} : \langle d_1, d_2, R_3 \rangle
  }
\]

\end{document}