\documentclass[preview]{standalone}
\usepackage{semantic}
\begin{document}
\[
  \inference[add]{
    F, D, L \vdash e_1 : \langle 1, 1, R \rangle \\
    F, D, L \vdash e_2 : \langle 1, 1, R \rangle \\
  }{
    F, D, L \vdash e_1 \texttt{ + } e_2 : \langle 1, 1, R \rangle
  }
\]

\[
  \inference[mul]{
    F, D, L \vdash e_1 : \langle 1, 1, R \rangle \\
    F, D, L \vdash e_2 : \langle 1, 1, R \rangle \\
  }{
    F, D, L \vdash e_1 \texttt{ * } e_2 : \langle 1, 1, R \rangle
  }
\]

\[
  \inference[sub]{
    F, D, L \vdash e_1 : \langle 1, 1, R \rangle \\
    F, D, L \vdash e_2 : \langle 1, 1, R \rangle \\
    R \in \{ \texttt{int}, \texttt{real}\} \\
  }{
    F, D, L \vdash e_1 \texttt{ - } e_2 : \langle 1, 1, R \rangle
  }
\]

\[
  \inference[div]{
    F, D, L \vdash e_1 : \langle 1, 1, \texttt{real} \rangle \\
    F, D, L \vdash e_2 : \langle 1, 1, \texttt{real} \rangle \\
  }{
    F, D, L \vdash e_1 \texttt{ / } e_2 : \langle 1, 1, \texttt{real} \rangle
  }
\]

\[
  \inference[neg]{
    F, D, L \vdash e : \langle 1, 1, R \rangle \\
    R \in \{ \texttt{int}, \texttt{real} \}
  }{
    F, D, L \vdash \texttt{-}\ e : \langle 1, 1, R \rangle
  }
\]

\[
  \inference[not]{
    F, D, L \vdash e : \langle 1, 1, \texttt{bool} \rangle \\
  }{
    F, D, L \vdash \texttt{!}\ e : \langle 1, 1, \texttt{bool} \rangle
  }
\]
\end{document}